wip

src/sequential/SeqLift.v
@@ -41,71 +41,70 @@ Definition update_flgas (f: flags) (l: Loc.t) (b: bool): flags :=
   fun l' => if (Loc.eq_dec l' l) then b else f l'.
 
 
-Definition sim_local (f_src: flags) (f_tgt: flags) (b: bool) (w: world) (views: Loc.t -> Time.t -> list View.t) (lc_src: Local.t) (lc_tgt: Local.t): Prop. Admitted.
+Definition sim_local (f_src: flags) (f_tgt: flags) (b: bool) (w: world) (lc_src: Local.t) (lc_tgt: Local.t): Prop. Admitted.
 
-Definition sim_memory (f_src: flags) (b: bool) (w: world) (views: Loc.t -> Time.t -> list View.t) (mem_src: Memory.t) (mem_tgt: Memory.t): Prop. Admitted.
+Definition sim_memory (f_src: flags) (b: bool) (w: world) (mem_src: Memory.t) (mem_tgt: Memory.t): Prop. Admitted.
 
 Definition sim_timemap: forall (w: world) (sc_src sc_tgt: TimeMap.t), Prop. Admitted.
 
-Lemma sim_local_future f_tgt w0 w1 views0 views1 lc_src lc_tgt
-      (SIM: sim_local flags_bot f_tgt false w0 views0 lc_src lc_tgt)
+Lemma sim_local_future f_tgt w0 w1 lc_src lc_tgt
+      (SIM: sim_local flags_bot f_tgt false w0 lc_src lc_tgt)
       (WORLD: world_messages_le (Messages.of_memory lc_src.(Local.promises)) w0 w1)
-      (VIEWS: views_le views0 views1)
   :
-    sim_local flags_bot f_tgt true w1 views1 lc_src lc_tgt.
+    sim_local flags_bot f_tgt true w1 lc_src lc_tgt.
 Admitted.
 
 Lemma sim_update_latest lang_src
       (st_src: lang_src.(Language.state))
-      f_tgt w views lc_src lc_tgt mem_src mem_tgt sc_src
-      (LOCAL: sim_local flags_bot f_tgt true w views lc_src lc_tgt)
-      (MEM: sim_memory flags_bot false w views mem_src mem_tgt)
+      f_tgt w lc_src lc_tgt mem_src mem_tgt sc_src
+      (LOCAL: sim_local flags_bot f_tgt true w lc_src lc_tgt)
+      (MEM: sim_memory flags_bot false w mem_src mem_tgt)
   :
     exists mem_src' lc_src',
       (<<STEPS: rtc (@Thread.tau_step _)
                     (Thread.mk _ st_src lc_src sc_src mem_src)
                     (Thread.mk _ st_src lc_src' sc_src mem_src')>>) /\
-      (<<LOCAL: sim_local flags_bot f_tgt false w views lc_src' lc_tgt>>) /\
-      (<<MEM: sim_memory flags_bot false w views mem_src' mem_tgt>>).
+      (<<LOCAL: sim_local flags_bot f_tgt false w lc_src' lc_tgt>>) /\
+      (<<MEM: sim_memory flags_bot false w mem_src' mem_tgt>>).
 Admitted.
 
-Lemma sim_cap f_tgt w0 views0 lc_src lc_tgt mem_src0 mem_tgt0 mem_tgt1
-      (LOCAL: sim_local flags_bot f_tgt false w0 views0 lc_src lc_tgt)
-      (MEM: sim_memory flags_bot false w0 views0 mem_src0 mem_tgt0)
+Lemma sim_cap f_tgt w0 lc_src lc_tgt mem_src0 mem_tgt0 mem_tgt1
+      (LOCAL: sim_local flags_bot f_tgt false w0 lc_src lc_tgt)
+      (MEM: sim_memory flags_bot false w0 mem_src0 mem_tgt0)
       (CAP: Memory.cap mem_tgt0 mem_tgt1)
   :
     exists tm_src mem_src1 w1,
       (<<TM: forall loc, Time.lt (Memory.max_ts loc mem_src0) (tm_src loc)>>) /\
       (<<CAP: CapFlex.cap_flex mem_src0 mem_src1 tm_src>>) /\
-      (<<MEM: sim_memory flags_bot true w1 views0 mem_src1 mem_tgt1>>) /\
-      (<<LOCAL: sim_local flags_bot f_tgt false w1 views0 lc_src lc_tgt>>) /\
-      (<<WORLD: world_messages_le (Messages.of_memory lc_src.(Local.promises)) w0 w1>>).
+      (<<MEM: sim_memory flags_bot true w1 mem_src1 mem_tgt1>>) /\
+      (<<LOCAL: sim_local flags_bot f_tgt false w1 lc_src lc_tgt>>) /\
+      (<<WORLD: world_messages_le (unchangable mem_src0 lc_src.(Local.promises)) w0 w1>>).
 Admitted.
 
-Lemma sim_local_lower flags_bot f_tgt w lc_src lc_tgt0 lc_tgt1 views
-      (SIM: sim_local flags_bot f_tgt false w views lc_src lc_tgt0)
+Lemma sim_local_lower flags_bot f_tgt w lc_src lc_tgt0 lc_tgt1
+      (SIM: sim_local flags_bot f_tgt false w lc_src lc_tgt0)
       (LOCAL: lower_local lc_tgt0 lc_tgt1)
   :
-    sim_local flags_bot f_tgt false w views lc_src lc_tgt1.
+    sim_local flags_bot f_tgt false w lc_src lc_tgt1.
 Admitted.
 
-Lemma sim_memory_lower f_src b w views mem_src mem_tgt0 mem_tgt1
-      (SIM: sim_memory f_src b w views mem_src mem_tgt0)
+Lemma sim_memory_lower f_src b w mem_src mem_tgt0 mem_tgt1
+      (SIM: sim_memory f_src b w mem_src mem_tgt0)
       (LOCAL: lower_memory mem_tgt0 mem_tgt1)
   :
-    sim_memory f_src b w views mem_src mem_tgt1.
+    sim_memory f_src b w mem_src mem_tgt1.
 Admitted.
 
-Lemma sim_cap f_tgt w0 views0 lc_src lc_tgt mem_src0 mem_tgt0 mem_tgt1
-      (LOCAL: sim_local flags_bot f_tgt false w0 views0 lc_src lc_tgt)
-      (MEM: sim_memory flags_bot false w0 views0 mem_src0 mem_tgt0)
+Lemma sim_make_promise f_tgt w0 lc_src lc_tgt mem_src0 mem_tgt0 mem_tgt1
+      (LOCAL: sim_local flags_bot f_tgt false w0 lc_src lc_tgt)
+      (MEM: sim_memory flags_bot false w0 mem_src0 mem_tgt0)
       (CAP: Memory.cap mem_tgt0 mem_tgt1)
   :
     exists tm_src mem_src1 w1,
       (<<TM: forall loc, Time.lt (Memory.max_ts loc mem_src0) (tm_src loc)>>) /\
       (<<CAP: CapFlex.cap_flex mem_src0 mem_src1 tm_src>>) /\
-      (<<MEM: sim_memory flags_bot true w1 views0 mem_src1 mem_tgt1>>) /\
-      (<<LOCAL: sim_local flags_bot f_tgt false w1 views0 lc_src lc_tgt>>) /\
+      (<<MEM: sim_memory flags_bot true w1 mem_src1 mem_tgt1>>) /\
+      (<<LOCAL: sim_local flags_bot f_tgt false w1 lc_src lc_tgt>>) /\
       (<<WORLD: world_messages_le (Messages.of_memory lc_src.(Local.promises)) w0 w1>>).
 Admitted.
 
@@ -125,6 +124,6 @@ Lemma sim_cap f_tgt w0 views0 lc_src lc_tgt mem_src0 mem_tgt0 mem_tgt1
       (<<WORLD: world_messages_le (Messages.of_memory lc_src.(Local.promises)) w0 w1>>).
 Admitted.
 
-Lemma sim_memory_promise
+(* Lemma sim_memory_promise *)
 
-Memory.promise
+(* Memory.promise *)
